Generalised corres proof for repeat
This commit contains a generalised proof about correspondence between
the generated C code for repeat and its update semantics embedding.

This commit also reorders and generalised the theorems for less than and
determinism on relations.

cogent/examples/repeat/RepeatCorres.thy
@@ -1,616 +1,558 @@
 theory RepeatCorres
   imports
-    RepeatAssm
+    RepeatUpdate
     CorresHelper
     CogentTypingHelper
+    "build/Generated_AllRefine"
 begin
-section "Corres"
 
+context update_sem_init begin
 
-context Generated_cogent_shallow begin
+definition crepeat
+  where
+"crepeat nC stopC stepC a0C o0C a1C a1U o1U d0 d1 a \<equiv>
+    do r <- select UNIV;
+       (i :: 64 word) <- gets (\<lambda>_. 0);
+       a0 <- select UNIV;
+       a0 <- gets (\<lambda>_. a1U (\<lambda>_. a0C a) a0);
+       a0 <- gets (\<lambda>_. o1U (\<lambda>_. o0C a) a0);
+       i <- gets (\<lambda>_. 0);
+       doE a0 <-
+           doE x <-
+               doE _ <- liftE (guard (\<lambda>s. True));
+                   whileLoopE (\<lambda>(ret, a0, i) s. i < ((nC a) :: 64 word))
+                     (\<lambda>(ret, a0, i).
+                         doE x <-
+                             doE retval <- liftE (do ret' <- d0 ((stopC a) :: 32 signed word) a0;
+                                                     gets (\<lambda>_. ret')
+                                                  od);
+                                 _ <- doE _ <- liftE (guard (\<lambda>s. True));
+                                          condition (\<lambda>s. boolean_C retval \<noteq> 0)
+                                            (doE global_exn_var <- liftE (gets (\<lambda>_. Break));
+                                                 throwError (global_exn_var, ret, a0)
+                                             odE)
+                                            (liftE (gets (\<lambda>_. ())))
+                                      odE;
+                                 liftE (do retval <- do ret' <- d1 ((stepC a) :: 32 signed word) a0;
+                                                        gets (\<lambda>_. ret')
+                                                     od;
+                                           a0 <- gets (\<lambda>_. a1U (\<lambda>_. retval) a0);
+                                           i <- gets (\<lambda>_. i + 1);
+                                           gets (\<lambda>_. (retval, a0, i))
+                                        od)
+                             odE;
+                             liftE
+                              (case x of
+                               (ret, a0, i) \<Rightarrow>
+                                 do _ <- guard (\<lambda>_. True);
+                                    gets (\<lambda>_. (ret, a0, i))
+                                 od)
+                         odE)
+                    (r, a0, i)
+               odE;
+               liftE (case x of (ret, a0, i) \<Rightarrow> gets (\<lambda>_. a0))
+           odE <handle2>
+           (\<lambda>(global_exn_var, ret, a0). doE _ <- doE _ <- liftE (guard (\<lambda>s. True));
+    condition (\<lambda>s. global_exn_var = Break)
+      (liftE (gets (\<lambda>_. ())))
+      (throwError ret)
+                                                                 odE;
+                                                            liftE (gets (\<lambda>_. a0))
+                                                        odE);
+           ret <- liftE (gets (\<lambda>_. a1C a0));
+           global_exn_var <- liftE (gets (\<lambda>_. Return));
+           throwError ret
+       odE <catch>
+       (\<lambda>ret. do _ <- gets (\<lambda>_. ());
+                 gets (\<lambda>_. ret)
+              od)
+    od"
 
-lemma dispatch_step:
-  "\<And>v' \<sigma> f g acc ra wa obsv ro b c j0 j.
-    \<lbrakk>proc_ctx_wellformed \<Xi>; val_rel g FUN_ENUM_log2step;
-     upd.uval_typing \<Xi> \<sigma> acc Generated_TypeProof.abbreviatedType1 ra wa; wa \<inter> ro = {};
-     upd.uval_typing \<Xi> \<sigma> obsv (TPrim (Num U64)) ro {}\<rbrakk> \<Longrightarrow>
-    \<lbrace>\<lambda>sa. j = j0 \<and>
-          b = c \<and> val_rel obsv (t2_C.obsv_C c) \<and> j < n_C v' \<and>
-          (\<exists>\<sigma>' y. urepeat_bod \<xi>_0 (unat j) (uvalfun_to_expr f) (uvalfun_to_expr g) \<sigma> \<sigma>'
-              Generated_TypeProof.abbreviatedType1 acc (TPrim (Num U64)) obsv y \<and>
-            (\<sigma>', sa) \<in> state_rel \<and> val_rel y (t2_C.acc_C c) \<and>
-            (\<xi>_0, [URecord [(y, type_repr (bang Generated_TypeProof.abbreviatedType1)), (obsv, RPrim (Num U64))]]
-                \<turnstile> (\<sigma>', App (uvalfun_to_expr f) (Var 0)) \<Down>! (\<sigma>', UPrim (LBool False))) \<and>
-            \<not>(\<xi>_0, [URecord [(y, type_repr (bang Generated_TypeProof.abbreviatedType1)), (obsv, RPrim (Num U64))]]
-                \<turnstile> (\<sigma>', App (uvalfun_to_expr f) (Var 0)) \<Down>! (\<sigma>', UPrim (LBool True))))\<rbrace>
-      dispatch_t4' FUN_ENUM_log2step c 
-    \<lbrace>\<lambda>y' sb. t2_C.acc_C_update (\<lambda>_. y') b = t2_C.acc_C_update (\<lambda>_. y') c \<and>
-            val_rel obsv (t2_C.obsv_C c) \<and>
-            j0 + 1 \<le> n_C v' \<and>
-            (\<exists>\<sigma>' y.
-              urepeat_bod \<xi>_0 (unat (j0 + 1)) (uvalfun_to_expr f) (uvalfun_to_expr g) \<sigma> \<sigma>'
-                Generated_TypeProof.abbreviatedType1 acc (TPrim (Num U64)) obsv y \<and>
-              (\<sigma>', sb) \<in> state_rel \<and> val_rel y y') \<and>
-            unat (n_C v') - unat (j0 + 1) < unat (n_C v') - unat j\<rbrace>!"
-  unfolding dispatch_t4'_def[simplified unknown_bind_ignore]
-  apply simp
+definition repeat_inv
+  where
+"repeat_inv srel \<xi>' (i :: 64 word) fstop fstep \<sigma> \<tau>a \<tau>o acc obsv s cn cacc cobsv \<equiv>
+    val_rel obsv cobsv \<and> i \<le> cn \<and>
+    (\<exists>\<sigma>' y. urepeat_bod \<xi>' (unat i) (uvalfun_to_expr fstop) (uvalfun_to_expr fstep) \<sigma> \<sigma>' \<tau>a acc \<tau>o obsv y \<and>
+            (\<sigma>', s) \<in> srel \<and> val_rel y cacc)"
+
+definition repeat_measure
+  where
+"repeat_measure i n = unat n - unat i"
+
+definition repeat_pre_step
+  where
+"repeat_pre_step srel \<xi>' i j fstop fstep \<sigma> \<tau>a \<tau>o acc obsv s cn cacc cobsv \<equiv> 
+    val_rel obsv cobsv \<and> i < cn \<and> i = j \<and> 
+    (\<exists>\<sigma>' y. urepeat_bod \<xi>' (unat i) (uvalfun_to_expr fstop) (uvalfun_to_expr fstep) \<sigma> \<sigma>' \<tau>a acc \<tau>o obsv y \<and>
+            (\<sigma>', s) \<in> srel \<and> val_rel y cacc \<and>
+            (\<xi>', [URecord [(y, type_repr (bang \<tau>a)), (obsv, type_repr \<tau>o)]]
+                \<turnstile> (\<sigma>', App (uvalfun_to_expr fstop) (Var 0)) \<Down>! (\<sigma>', UPrim (LBool False))))"
+
+lemma step_wp:
+  assumes \<Xi>wellformed: "proc_ctx_wellformed \<Xi>'"
+  and     \<xi>'matchesu: "\<xi>' matches-u \<Xi>'"
+  and     determ: "determ \<xi>'"
+  and     \<tau>fdef: "\<tau>f = TRecord [(''acc'', \<tau>a, Present), (''obsv'', \<tau>o, Present)] Unboxed"
+  and     fsteptype: "\<Xi>', [], [Some \<tau>f] \<turnstile> App (uvalfun_to_expr fstep) (Var 0) : \<tau>a"
+  and     valrelc:  "\<And>x x'. val_rel x (x' :: ('c :: cogent_C_val)) \<equiv>
+                              \<exists>acc obsv. x = URecord [acc, obsv] \<and> val_rel (fst acc) (a1C x') \<and>
+                                val_rel (fst obsv) (o1C x')"
+  and     d1corres: "\<And>x x' \<sigma> s. val_rel x (x' :: ('c :: cogent_C_val)) \<Longrightarrow>
+                                  corres state_rel (App (uvalfun_to_expr fstep) (Var 0))
+                                    (do ret <- d1 (stepC v') x'; gets (\<lambda>s. ret) od)
+                                    \<xi>' [x] \<Xi>' [option.Some \<tau>f] \<sigma> s"
+  and     a1C_a1U: "\<And>x y. a1C (a1U (\<lambda>_. y) x) = y"
+  and     o1C_a1U: "\<And>x y. o1C (a1U y x) = o1C x"
+  and     srel: "(\<sigma>, s) \<in> state_rel"
+  and     acctyp: "\<Xi>', \<sigma> \<turnstile> acc :u \<tau>a \<langle>ra, wa\<rangle>"
+  and     obsvtyp: "\<Xi>', \<sigma> \<turnstile> obsv :u \<tau>o \<langle>ro, {}\<rangle>"
+  and     disjoint: "wa \<inter> ro = {}"
+  and     valrelacc: "val_rel acc (a0C v')"
+  and     valrelobsv: "val_rel obsv (o0C v')"
+  shows "\<And>arg j i.
+          \<lbrace>\<lambda>sa. repeat_pre_step state_rel \<xi>' i j fstop fstep \<sigma> \<tau>a \<tau>o acc obsv sa (nC v') (a1C arg) (o1C arg)\<rbrace>
+            d1 (stepC v') arg 
+          \<lbrace>\<lambda>ret sb.
+               repeat_inv state_rel \<xi>' (j + 1) fstop fstep \<sigma> \<tau>a \<tau>o acc obsv sb (nC v') (a1C (a1U (\<lambda>_. ret) arg))
+                (o1C (a1U (\<lambda>_. ret) arg)) \<and>
+               repeat_measure (j+1) (nC v') < repeat_measure i (nC v')\<rbrace>!"
   apply (clarsimp simp: validNF_def valid_def no_fail_def)
   apply (subst all_imp_conj_distrib[symmetric]; clarsimp)
+  apply (clarsimp simp: repeat_pre_step_def repeat_inv_def repeat_measure_def)
   apply (rename_tac s \<sigma>' y)
-  apply (cut_tac \<sigma> = \<sigma>' and s = s and a' = c and
-      a = "URecord [(y, type_repr Generated_TypeProof.abbreviatedType1),
-            (obsv, type_repr (TPrim (Num U64)))]" in corres_log2step[simplified \<Xi>_def[symmetric]])
-   apply (clarsimp simp: val_rel_simp)
-  apply (clarsimp simp: corres_def)
-  apply (erule impE, rule \<xi>_0_matchesu_\<Xi>)
-  apply (frule_tac \<xi>' = \<xi>_0  and ro = ro and ra = ra and wa = wa and obsv = obsv and acc = acc
-      in upd.urepeat_bod_preservation; simp?)
-     apply (rule \<xi>_0_matchesu_\<Xi>)
-    apply blast
-   apply (clarsimp simp: val_rel_fun_tag cogent_function_val_rel untyped_func_enum_defs)
-   apply (intro conjI typing_mono_app_cogent_fun; clarsimp simp: abbreviated_type_defs)
-   apply (rule log2step_typecorrect'[simplified snd_conv fst_conv log2step_type_def abbreviated_type_defs])
-  apply clarsimp
-  apply (rename_tac r' w')
-  apply (erule impE)
+  apply (insert d1corres)
+  apply (drule_tac x = "URecord [(y, type_repr \<tau>a), (obsv, type_repr \<tau>o)]" and
+                   y = arg in meta_spec2)
+  apply (drule_tac x = \<sigma>' and y = s in meta_spec2)
+  apply (erule meta_impE)
+   apply (simp add: valrelc)
+  apply (clarsimp simp: corres_def \<Xi>wellformed \<xi>'matchesu)
+  apply (erule impE) 
+   apply (drule urepeat_bod_preservation[OF \<Xi>wellformed \<xi>'matchesu acctyp obsvtyp
+                                            disjoint[simplified Int_commute] _
+                                            fsteptype[simplified \<tau>fdef]])
+   apply clarsimp
+   apply (rename_tac r' w')
    apply (rule_tac x = "r' \<union> ro" in exI)
    apply (rule_tac x = w' in exI)
-   apply (simp add: log2step_type_def abbreviated_type_defs)
-   apply (intro upd.matches_ptrs_some[where r' = "{}" and w' = "{}", simplified]
-      upd.matches_ptrs_empty[where \<tau>s = "[]", simplified]
-      upd.u_t_struct
-      upd.u_t_r_cons1[where w' = "{}", simplified]
-      upd.u_t_r_cons1[where r' = "{}" and w' = "{}", simplified]
-      upd.u_t_r_empty; simp?)
-    apply (drule_tac u = obsv in upd.uval_typing_frame(1); simp?)
-    apply blast
-   apply (drule_tac v = obsv in upd.frame_noalias_uval_typing'(2); simp?)
-    apply blast
-   apply blast
+   apply (clarsimp simp: \<tau>fdef)
+   apply (intro matches_ptrs_some[where r' = "{}" and w' = "{}", simplified]
+                matches_ptrs_empty[where \<tau>s = "[]", simplified]
+                u_t_struct
+                u_t_r_cons1[where w' = "{}", simplified]
+                u_t_r_cons1[where r' = "{}" and w' = "{}", simplified]
+                u_t_r_empty; simp?)
+    apply (erule uval_typing_frame(1); simp add: obsvtyp disjoint[simplified Int_commute])
+   apply (drule frame_noalias_uval_typing'(2)[OF _ obsvtyp disjoint[simplified Int_commute]]; blast)
   apply clarsimp
-  apply (rename_tac res s')
-  apply (erule_tac x = res in allE)
-  apply (erule_tac x = s' in allE)
-  apply clarsimp
-  apply (rule conjI)
-   apply unat_arith
-  apply (simp only: less_is_non_zero_p1[THEN  unatSuc2])
-  apply (rule conjI)
-   apply (intro exI conjI; assumption?)
-   apply (rule upd.urepeat_bod_step; simp?)
-   apply (simp add: val_rel_fun_tag cogent_function_val_rel untyped_func_enum_defs)
-   apply (rule u_sem_app[where ts ="[]" and y = "Var 0" and \<gamma> = "[_]",
-        simplified,OF _ u_sem_var, simplified]; simp?)
-   apply (intro u_sem_fun)
-  apply unat_arith
+  apply (rename_tac a b)
+  apply (elim allE impE, assumption)
+  apply (clarsimp simp: inc_le)
+  apply (simp only: less_is_non_zero_p1[THEN unatSuc2] word_less_nat_alt)
+  apply (frule urepeat_bod_step_determ[OF _ _ _ determ]; (simp del: urepeat_bod.simps)?)
+  apply (intro conjI exI; assumption?; (simp del: urepeat_bod.simps add: o1C_a1U a1C_a1U)?)
   done
 
-lemma log2stop_deterministic:
-  "\<lbrakk>\<xi>_0, [URecord [(a, f), (b, g)]] \<turnstile> (\<sigma>, Generated_TypeProof.log2stop) \<Down>! (\<sigma>', c); d \<noteq> c\<rbrakk>
-    \<Longrightarrow> \<not>(\<xi>_0, [URecord [(a, f), (b, g)]] \<turnstile> (\<sigma>, App (Fun Generated_TypeProof.log2stop []) (Var 0)) \<Down>! (\<sigma>'', d))"
-  "\<lbrakk>\<xi>_0, [URecord [(a, f), (b, g)]] \<turnstile> (\<sigma>, Generated_TypeProof.log2stop) \<Down>! (\<sigma>', c); \<sigma>' \<noteq> \<sigma>''\<rbrakk>
-    \<Longrightarrow> \<not>(\<xi>_0, [URecord [(a, f), (b, g)]] \<turnstile> (\<sigma>, App (Fun Generated_TypeProof.log2stop []) (Var 0)) \<Down>! (\<sigma>'', d))"
-  unfolding log2stop_def abbreviatedType1_def
-  apply (fastforce elim: u_sem_takeE u_sem_appE u_sem_funE u_sem_afunE u_sem_primE u_sem_consE)+
-  done
-
-lemma dispatch_stop:
-  "\<And>v' \<sigma> f g acc ra wa obsv ro j b c j'.
-    \<lbrakk>proc_ctx_wellformed \<Xi>; val_rel f FUN_ENUM_log2stop; val_rel g FUN_ENUM_log2step;
-     upd.uval_typing \<Xi> \<sigma> acc Generated_TypeProof.abbreviatedType1 ra wa; wa \<inter> ro = {};
-     upd.uval_typing \<Xi> \<sigma> obsv (TPrim (Num U64)) ro {}\<rbrakk> \<Longrightarrow>
-    \<lbrace>\<lambda>sa. (\<exists>\<sigma>' y n. (\<sigma>', sa) \<in> state_rel \<and> val_rel y (t2_C.acc_C c) \<and> val_rel obsv (t2_C.obsv_C c) \<and>
-            j = j' \<and> b = c \<and> j < n_C v' \<and>
-            urepeat_bod \<xi>_0 n (uvalfun_to_expr f) (uvalfun_to_expr g) \<sigma> \<sigma>'
-              Generated_TypeProof.abbreviatedType1 acc (TPrim (Num U64)) obsv y \<and>
-            ((\<xi>_0 , [URecord [(y, type_repr (bang Generated_TypeProof.abbreviatedType1)),
-                (obsv, type_repr (TPrim (Num U64)))]]
-                \<turnstile> (\<sigma>', App (uvalfun_to_expr f) (Var 0)) \<Down>! (\<sigma>', UPrim (LBool True))) \<and>
-             \<not>(\<xi>_0 , [URecord [(y, type_repr (bang Generated_TypeProof.abbreviatedType1)),
-                (obsv, type_repr (TPrim (Num U64)))]]
-                \<turnstile> (\<sigma>', App (uvalfun_to_expr f) (Var 0)) \<Down>! (\<sigma>', UPrim (LBool False)))
-              \<longrightarrow> n \<ge> unat j \<and> n < unat (n_C v')) \<and>
-            ((\<xi>_0 , [URecord [(y, type_repr (bang Generated_TypeProof.abbreviatedType1)),
-                (obsv, type_repr (TPrim (Num U64)))]]
-                \<turnstile> (\<sigma>', App (uvalfun_to_expr f) (Var 0)) \<Down>! (\<sigma>', UPrim (LBool False))) \<and>
-             \<not>(\<xi>_0 , [URecord [(y, type_repr (bang Generated_TypeProof.abbreviatedType1)),
-                (obsv, type_repr (TPrim (Num U64)))]]
-                \<turnstile> (\<sigma>', App (uvalfun_to_expr f) (Var 0)) \<Down>! (\<sigma>', UPrim (LBool True)))
+lemma stop_wp:
+  assumes \<Xi>wellformed: "proc_ctx_wellformed \<Xi>'"
+  and     \<xi>'matchesu: "\<xi>' matches-u \<Xi>'"
+  and     determ: "determ \<xi>'"
+  and     \<tau>fdef: "\<tau>f = TRecord [(''acc'', \<tau>a, Present), (''obsv'', \<tau>o, Present)] Unboxed"
+  and     fstoptype: "\<Xi>', [], [Some (bang \<tau>f)] \<turnstile> App (uvalfun_to_expr fstop) (Var 0) : TPrim Bool"
+  and     fsteptype: "\<Xi>', [], [Some \<tau>f] \<turnstile> App (uvalfun_to_expr fstep) (Var 0) : \<tau>a"
+  and     valrelc:  "\<And>x x'. val_rel x (x' :: ('c :: cogent_C_val)) \<equiv>
+                              \<exists>acc obsv. x = URecord [acc, obsv] \<and> val_rel (fst acc) (a1C x') \<and>
+                                val_rel (fst obsv) (o1C x')"
+  and     d0corres: "\<And>x x' \<sigma> s. val_rel x (x' :: ('c :: cogent_C_val)) \<Longrightarrow>
+                                  corres state_rel (App (uvalfun_to_expr fstop) (Var 0))
+                                    (do ret <- d0 (stopC v') x'; gets (\<lambda>s. ret) od)
+                                    \<xi>' [x] \<Xi>' [option.Some (bang \<tau>f)] \<sigma> s"
+  and     srel: "(\<sigma>, s) \<in> state_rel"
+  and     acctyp: "\<Xi>', \<sigma> \<turnstile> acc :u \<tau>a \<langle>ra, wa\<rangle>"
+  and     obsvtyp: "\<Xi>', \<sigma> \<turnstile> obsv :u \<tau>o \<langle>ro, {}\<rangle>"
+  and     disjoint: "wa \<inter> ro = {}"
+  and     valrelacc: "val_rel acc (a0C v')"
+  and     valrelobsv: "val_rel obsv (o0C v')"
+  shows "\<And>j arg j'.
+          \<lbrace>\<lambda>sa. (\<exists>\<sigma>' y n. (\<sigma>', sa) \<in> state_rel \<and> val_rel y (a1C arg) \<and> val_rel obsv (o1C arg) \<and>
+            j = j' \<and>  j < nC v' \<and>
+            urepeat_bod \<xi>' n (uvalfun_to_expr fstop) (uvalfun_to_expr fstep) \<sigma> \<sigma>'
+              \<tau>a acc \<tau>o obsv y \<and>
+            ((\<xi>' , [URecord [(y, type_repr (bang \<tau>a)), (obsv, type_repr \<tau>o)]]
+                \<turnstile> (\<sigma>', App (uvalfun_to_expr fstop) (Var 0)) \<Down>! (\<sigma>', UPrim (LBool True)))
+              \<longrightarrow> n \<ge> unat j \<and> n < unat (nC v')) \<and>
+            ((\<xi>' , [URecord [(y, type_repr (bang \<tau>a)), (obsv, type_repr \<tau>o)]]
+                \<turnstile> (\<sigma>', App (uvalfun_to_expr fstop) (Var 0)) \<Down>! (\<sigma>', UPrim (LBool False)))
               \<longrightarrow> n = unat j))\<rbrace>
-      dispatch_t3' FUN_ENUM_log2stop b 
-    \<lbrace>\<lambda>x sb.
-        (boolean_C x \<noteq> 0 \<longrightarrow>
-            (\<exists>\<sigma>' y.
-              urepeat_bod \<xi>_0 (unat (n_C v')) (uvalfun_to_expr f) (uvalfun_to_expr g) \<sigma> \<sigma>'
-                Generated_TypeProof.abbreviatedType1 acc (TPrim (Num U64)) obsv y \<and>
-              (\<sigma>', sb) \<in> state_rel \<and> val_rel y (t2_C.acc_C c))) \<and>
-        (boolean_C x = 0 \<longrightarrow>
-            j = j' \<and>
-            b = c \<and>
-            val_rel obsv (t2_C.obsv_C c) \<and>
-            j < n_C v' \<and>
-            (\<exists>\<sigma>' y.
-              urepeat_bod \<xi>_0 (unat j) (uvalfun_to_expr f) (uvalfun_to_expr g) \<sigma> \<sigma>'
-                Generated_TypeProof.abbreviatedType1 acc (TPrim (Num U64)) obsv y \<and>
-              (\<sigma>', sb) \<in> state_rel \<and> val_rel y (t2_C.acc_C c) \<and>
-               (\<xi>_0, [URecord [(y, type_repr (bang Generated_TypeProof.abbreviatedType1)), (obsv, RPrim (Num U64))]]
-                \<turnstile> (\<sigma>', App (uvalfun_to_expr f) (Var 0)) \<Down>! (\<sigma>', UPrim (LBool False))) \<and>
-              \<not>(\<xi>_0, [URecord [(y, type_repr (bang Generated_TypeProof.abbreviatedType1)), (obsv, RPrim (Num U64))]]
-                \<turnstile> (\<sigma>', App (uvalfun_to_expr f) (Var 0)) \<Down>! (\<sigma>', UPrim (LBool True)))))\<rbrace>!"
-  unfolding dispatch_t3'_def[simplified unknown_bind_ignore]
-  apply simp
+            d0 (stopC v') arg 
+           \<lbrace>\<lambda>ret sb.
+               (boolean_C ret \<noteq> 0 \<longrightarrow>
+                (\<exists>\<sigma>' y.
+                    urepeat_bod \<xi>' (unat (nC v')) (uvalfun_to_expr fstop) (uvalfun_to_expr fstep) \<sigma> \<sigma>' \<tau>a acc \<tau>o obsv y \<and>
+                    (\<sigma>', sb) \<in> state_rel \<and> val_rel y (a1C arg))) \<and>
+               (boolean_C ret = 0 \<longrightarrow>
+                repeat_pre_step state_rel \<xi>' j j' fstop fstep \<sigma> \<tau>a \<tau>o acc obsv sb (nC v') (a1C arg) (o1C arg))\<rbrace>!"
   apply (clarsimp simp: validNF_def valid_def no_fail_def)
   apply (subst all_imp_conj_distrib[symmetric]; clarsimp)
+  apply (clarsimp simp: repeat_pre_step_def)
   apply (rename_tac s \<sigma>' y n)
-  apply (cut_tac \<sigma> = \<sigma>' and s = s and a' = c and
-      a = "URecord [(y, type_repr Generated_TypeProof.abbreviatedType1),
-            (obsv, type_repr (TPrim (Num U64)))]" in corres_log2stop[simplified \<Xi>_def[symmetric]])
-   apply (clarsimp simp: val_rel_simp)
-  apply (clarsimp simp: corres_def)
-  apply (erule impE, rule \<xi>_0_matchesu_\<Xi>)
- apply (frule_tac \<xi>' = \<xi>_0  and ro = ro and ra = ra and wa = wa and obsv = obsv and acc = acc
-      in upd.urepeat_bod_preservation; simp?)
-     apply (rule \<xi>_0_matchesu_\<Xi>)
-    apply blast
-   apply (clarsimp simp: val_rel_fun_tag cogent_function_val_rel untyped_func_enum_defs)
-   apply (intro conjI typing_mono_app_cogent_fun; clarsimp simp: abbreviated_type_defs)
-   apply (rule log2step_typecorrect'[simplified snd_conv fst_conv log2step_type_def abbreviated_type_defs])
+  apply (insert d0corres)
+  apply (drule_tac x = "URecord [(y, type_repr (bang \<tau>a)), (obsv, type_repr \<tau>o)]" and
+                   y = arg in meta_spec2)
+  apply (drule_tac x = \<sigma>' and y = s in meta_spec2)
+  apply (erule meta_impE)
+   apply (simp add: valrelc)
+  apply (clarsimp simp: corres_def \<Xi>wellformed \<xi>'matchesu)
+  apply (frule urepeat_bod_preservation[OF \<Xi>wellformed \<xi>'matchesu acctyp obsvtyp
+                                           disjoint[simplified Int_commute] _
+                                           fsteptype[simplified \<tau>fdef]])
   apply clarsimp
   apply (rename_tac r' w')
-  apply (erule impE, rule_tac x = "r' \<union> ro" in exI)
-   apply (rule_tac x = w' in exI)
-  apply (simp add: log2stop_type_def abbreviated_type_defs)
-   apply (intro upd.matches_ptrs_some[where r' = "{}" and w' = "{}", simplified]
-      upd.matches_ptrs_empty[where \<tau>s = "[]", simplified]
-      upd.u_t_struct
-      upd.u_t_r_cons1[where w' = "{}", simplified]
-      upd.u_t_r_cons1[where r' = "{}" and w' = "{}", simplified]
-      upd.u_t_r_empty; simp?)
-    apply (drule_tac u = obsv in upd.uval_typing_frame(1); simp?)
-    apply blast
-   apply (drule_tac v = obsv in upd.frame_noalias_uval_typing'(2); simp?)
-    apply blast
-   apply blast
+  apply (erule impE, rule_tac x = "(r' \<union> w') \<union> ro" in exI, rule_tac x = "{}" in exI) 
+   apply (clarsimp simp: \<tau>fdef)
+   apply (intro matches_ptrs_some[where r' = "{}" and w' = "{}", simplified]
+                matches_ptrs_empty[where \<tau>s = "[]", simplified]
+                u_t_struct
+                u_t_r_cons1[where w' = "{}", simplified]
+                u_t_r_cons1[where r' = "{}" and w' = "{}", simplified]
+                u_t_r_empty; simp?)
+     apply (rule uval_typing_bang(1); simp)
+    apply (rule uval_typing_bang(1)[where w = "{}" ,simplified])
+    apply (erule uval_typing_frame(1); simp add: obsvtyp disjoint[simplified Int_commute])
+   apply (rule wellformed_imp_bang_type_repr[OF uval_typing_to_wellformed(1)[OF obsvtyp]])
   apply clarsimp
-  apply (rename_tac res s')
-  apply (erule_tac x = res in allE)
-  apply (erule_tac x = s' in allE)
-  apply clarsimp 
-  apply (drule_tac w = "{}" and r = "(r' \<union> w') \<union> ro" and \<tau> = "TPrim Bool" and
-      ?\<Gamma>.0 = "[option.Some Generated_TypeProof.abbreviatedType2]"
-      in upd.preservation_mono(1)[OF _ _  \<xi>_0_matchesu_\<Xi>]; simp?)
-    apply (drule_tac v = y in upd.uval_typing_bang(1))
-    apply (clarsimp simp: abbreviated_type_defs)
-    apply (intro upd.matches_ptrs_some[where r' = "{}" and w' = "{}", simplified]
-      upd.matches_ptrs_empty[where \<tau>s = "[]", simplified]
-      upd.u_t_struct
-      upd.u_t_r_cons1[where w' = "{}", simplified]
-      upd.u_t_r_cons1[where r' = "{}" and w' = "{}", simplified]
-      upd.u_t_r_empty; simp?)
-    apply (drule_tac u = obsv in upd.uval_typing_frame(1); simp?)
-    apply blast
-   apply (drule_tac v = obsv in upd.frame_noalias_uval_typing'(2); simp?)
-    apply blast
-   apply (rule log2stop_typecorrect'[simplified fst_conv snd_conv log2stop_type_def])
+  apply (rename_tac a b)
+  apply (elim allE, erule impE, assumption)
   apply clarsimp
-  apply (frule_tac v = r in upd.tprim_no_pointers(1))
-  apply (drule_tac v = r in upd.tprim_no_pointers(2))
-  apply clarsimp
-  apply (drule upd.frame_empty; clarsimp)
-  apply (rule conjI; clarsimp simp: val_rel_bool_t_C_def)
-  apply (erule impE)
-    apply (clarsimp simp: val_rel_fun_tag cogent_function_val_rel untyped_func_enum_defs abbreviated_type_defs)
-    apply (rule conjI)
-     apply (rule u_sem_app[where ts ="[]" and y = "Var 0" and \<gamma> = "[_]",
-        simplified,OF _ u_sem_var, simplified]; simp?)
-     apply (intro u_sem_fun)
-    apply (drule_tac d = "UPrim (LBool False)" and \<sigma>'' = \<sigma>'' in log2stop_deterministic(1);simp)
-   apply (intro exI conjI; simp?)
-   apply (rule_tac i = n in upd.urepeat_bod_early_termination; simp add: word_less_nat_alt)
-   apply (clarsimp simp: val_rel_fun_tag cogent_function_val_rel untyped_func_enum_defs abbreviated_type_defs)
-   apply (rule u_sem_app[where ts ="[]" and y = "Var 0" and \<gamma> = "[_]",
-        simplified,OF _ u_sem_var, simplified]; simp?)
-    apply (intro u_sem_fun)
-  apply (thin_tac "_ \<longrightarrow> _")
-  apply (clarsimp simp: val_rel_fun_tag cogent_function_val_rel untyped_func_enum_defs abbreviated_type_defs)
-  apply (frule_tac d = "UPrim (LBool True)" and \<sigma>'' = \<sigma>'' in log2stop_deterministic(1);simp)
-  apply (erule impE)
-   apply (rule u_sem_app[where ts ="[]" and y = "Var 0" and \<gamma> = "[_]",
-        simplified,OF _ u_sem_var, simplified]; simp?)
-   apply (intro u_sem_fun)
-  apply (intro exI conjI; simp)
-  apply (rule u_sem_app[where ts ="[]" and y = "Var 0" and \<gamma> = "[_]",
-        simplified,OF _ u_sem_var, simplified]; simp?)
-  apply (intro u_sem_fun)
+  apply (frule_tac r = "(r' \<union> w') \<union> ro" and w = "{}" 
+      in preservation(1)[where K = "[]" and \<tau>s = "[]", simplified,
+                         OF \<Xi>wellformed _ \<xi>'matchesu _ fstoptype, rotated 1])
+   apply (clarsimp simp: \<tau>fdef)
+   apply (intro matches_ptrs_some[where r' = "{}" and w' = "{}", simplified]
+                matches_ptrs_empty[where \<tau>s = "[]", simplified]
+                u_t_struct
+                u_t_r_cons1[where w' = "{}", simplified]
+                u_t_r_cons1[where r' = "{}" and w' = "{}", simplified]
+                u_t_r_empty; simp?)
+     apply (rule uval_typing_bang(1); simp)
+    apply (rule uval_typing_bang(1)[where w = "{}" ,simplified])
+    apply (erule uval_typing_frame(1); simp add: obsvtyp disjoint[simplified Int_commute])
+   apply (rule wellformed_imp_bang_type_repr[OF uval_typing_to_wellformed(1)[OF obsvtyp]])
+  apply (clarsimp simp: val_rel_bool_t_C_def)
+  apply (erule u_t_primE; clarsimp)
+  apply (drule frame_empty; clarsimp)
+  apply (rule conjI; clarsimp)
+  apply (intro exI conjI; assumption?)
+   apply (erule (2) urepeat_bod_early_termination)
+  apply (intro exI conjI; assumption?)
   done
 
-
-lemma repeat_corres:
-  "\<And>v' i \<gamma> \<Gamma> \<sigma> s.
-    \<lbrakk>stop_C v' = FUN_ENUM_log2stop; step_C v' = FUN_ENUM_log2step; i < length \<gamma>; val_rel (\<gamma> ! i) v';
-     \<Gamma> ! i = Some (fst (snd repeat_0_type))\<rbrakk>
-    \<Longrightarrow> corres state_rel (App (AFun ''repeat_0'' []) (Var i)) (do x <- repeat_0' v';
- gets (\<lambda>s. x)
-                                                               od)
-         \<xi>_1 \<gamma> \<Xi> \<Gamma> \<sigma> s"
-  apply (rule absfun_corres; simp?)
-   prefer 2
-  \<comment>\<open>For automation, make a repeat_type_defs lemma\<close>
-   apply (clarsimp simp: repeat_0_type_def abbreviated_type_defs \<Xi>_def)
-  apply (subst abs_fun_rel_def'; clarsimp)
-  apply (rotate_tac -1)
-  apply (subst (asm) \<Xi>_def; clarsimp)
-  apply (clarsimp simp: repeat_0_type_def)
-  apply (subst (asm) val_rel_simp; clarsimp)
-  apply (rename_tac r w n rn f rf g rg acc racc obsv robsv)
-  apply (subst (asm) val_rel_word64; clarsimp)
-  apply (erule upd.u_t_recE; clarsimp)
-  apply (erule upd.u_t_r_consE; clarsimp)+
-  apply (erule upd.u_t_r_emptyE; clarsimp)
-  apply (frule upd.tprim_no_pointers(1); clarsimp)
-  apply (frule upd.tprim_no_pointers(2); clarsimp)
-  apply (frule upd.tfun_no_pointers(1); clarsimp)
-  apply (drule upd.tfun_no_pointers(2); clarsimp)
-  apply (frule upd.tfun_no_pointers(1); clarsimp)
-  apply (drule upd.tfun_no_pointers(2); clarsimp)
-  apply (rename_tac f g acc ra wa obsv ro wo)
-  apply (frule_tac v = obsv and K' = "[]" in upd.discardable_or_shareable_not_writable'(1)[rotated 2]; simp?)
-    apply (rule kindingI; simp)
-   apply blast
-  apply clarsimp
-  unfolding repeat_0'_def
-  apply (clarsimp simp: L2polish unknown_bind_ignore)
-  apply (subst \<xi>1_def; clarsimp simp: urepeat_def)
-  apply (subgoal_tac "is_uvalfun f \<and>
-               is_uvalfun g \<and>
-               \<Xi>, [], [Some (TRecord
-                               [(''acc'', bang Generated_TypeProof.abbreviatedType1, Present),
-                                (''obsv'', TPrim (Num U64), Present)]
-                               Unboxed)] \<turnstile> App (uvalfun_to_expr f) (Var 0) : TPrim Bool \<and>
-               \<Xi>, [], [Some (TRecord
-                               [(''acc'', Generated_TypeProof.abbreviatedType1, Present), (''obsv'', TPrim (Num U64), Present)]
-                               Unboxed)] \<turnstile> App (uvalfun_to_expr g) (Var 0) : Generated_TypeProof.abbreviatedType1")
-   apply simp
-   apply (thin_tac "_ \<and> _ \<and> _ \<and> _")
-   defer
-   apply (clarsimp simp: val_rel_simp cogent_function_val_rel untyped_func_enum_defs)
-   apply (intro conjI typing_mono_app_cogent_fun; clarsimp simp: abbreviated_type_defs)
-    apply (rule log2stop_typecorrect'[simplified snd_conv fst_conv log2stop_type_def abbreviated_type_defs])
-   apply (rule log2step_typecorrect'[simplified snd_conv fst_conv log2step_type_def abbreviated_type_defs])
-  apply (wp; (clarsimp split: prod.splits)?)
-     apply (rename_tac breakval)
+lemma crepeat_corres_base:
+  assumes \<gamma>len: "i < length \<gamma>"
+  and     valrel: "val_rel (\<gamma> ! i) (v' :: ('a :: cogent_C_val))"
+  and     \<Gamma>i: "\<Gamma> ! i = Some (fst (snd (\<Xi>' name)))"
+  and     \<Xi>name: "\<Xi>' name = ([], \<tau>, \<tau>a)"
+  and     \<tau>def: "\<tau> = TRecord [(''n'', TPrim (Num U64), Present),
+                              (''stop'', TFun (bang \<tau>f) (TPrim Bool), Present),
+                              (''step'', TFun \<tau>f \<tau>a, Present),
+                              (''acc'', \<tau>a, Present), (''obsv'', \<tau>o, Present)] Unboxed"
+  and     \<tau>fdef: "\<tau>f = TRecord [(''acc'', \<tau>a, Present), (''obsv'', \<tau>o, Present)] Unboxed"
+  and     bang\<tau>o: "bang \<tau>o = \<tau>o"
+  and     \<xi>''name: "\<xi>'' name = urepeat \<Xi>' \<xi>' \<tau>a \<tau>o"
+  and     \<xi>'matchesu: "\<xi>' matches-u \<Xi>'"
+  and     determ: "determ \<xi>'"
+  and     \<gamma>i: "\<gamma> ! i = URecord [(UPrim (LU64 n), RPrim (Num U64)), (fstop, RFun), (fstep, RFun), (acc, type_repr \<tau>a), (obsv, type_repr \<tau>o)]"
+  and     fstoptype: "\<Xi>', [], [Some (bang \<tau>f)] \<turnstile> App (uvalfun_to_expr fstop) (Var 0) : TPrim Bool"
+  and     fsteptype: "\<Xi>', [], [Some \<tau>f] \<turnstile> App (uvalfun_to_expr fstep) (Var 0) : \<tau>a"
+  and     d0corres: "\<And>x x' \<sigma> s. val_rel x (x' :: ('c :: cogent_C_val)) \<Longrightarrow>
+                                  corres state_rel (App (uvalfun_to_expr fstop) (Var 0))
+                                    (do ret <- d0 (stopC v') x'; gets (\<lambda>s. ret) od)
+                                    \<xi>' [x] \<Xi>' [option.Some (bang \<tau>f)] \<sigma> s"
+  and     d1corres: "\<And>x x' \<sigma> s. val_rel x x' \<Longrightarrow>
+                                  corres state_rel (App (uvalfun_to_expr fstep) (Var 0))
+                                    (do ret <- d1 (stepC v') x'; gets (\<lambda>s. ret) od)
+                                    \<xi>' [x] \<Xi>' [option.Some \<tau>f] \<sigma> s"
+  and     valrela:  "\<And>x x'. val_rel x (x' :: 'a) \<equiv>
+                              \<exists>n f g acc obsv. x = URecord [n, f, g, acc, obsv] \<and>
+                                val_rel (fst n) (nC x') \<and> val_rel (fst f) (stopC x') \<and>
+                                val_rel (fst g) (stepC x') \<and> val_rel (fst acc) (a0C x') \<and>
+                                val_rel (fst obsv) (o0C x')"
+  and     valrelc:  "\<And>x x'. val_rel x (x' :: 'c) \<equiv>
+                              \<exists>acc obsv. x = URecord [acc, obsv] \<and> val_rel (fst acc) (a1C x') \<and>
+                                val_rel (fst obsv) (o1C x')"
+  and     a1C_a1U: "\<And>x y. a1C (a1U (\<lambda>_. y) x) = y"
+  and     a1C_o1U: "\<And>x y. a1C (o1U y x) = a1C x"
+  and     o1C_o1U: "\<And>x y. o1C (o1U (\<lambda>_. y) x) = y"
+  and     o1C_a1U: "\<And>x y. o1C (a1U y x) = o1C x"
+  and     cfundef: "cfun = crepeat nC stopC stepC a0C o0C a1C a1U o1U d0 d1"
+shows
+  "corres state_rel (App (AFun name []) (Var i))
+    (do x <- cfun v'; gets (\<lambda>s. x) od)
+     \<xi>'' \<gamma> \<Xi>' \<Gamma> \<sigma> s"
+proof (rule absfun_corres[OF _ \<gamma>len valrel])
+  show "abs_fun_rel \<Xi>' state_rel name \<xi>'' cfun \<sigma> s (\<gamma> ! i) v'"
+    apply (subst abs_fun_rel_def')
+    apply (clarsimp simp: \<Xi>name \<tau>def \<xi>''name cfundef urepeat_def bang\<tau>o \<gamma>i fsteptype[simplified \<tau>fdef])
+    apply (insert fstoptype; simp add: \<tau>fdef bang\<tau>o)
+    apply (thin_tac "_, _, _ \<turnstile> _ : _")
+    apply (erule u_t_recE; clarsimp)
+    apply (erule u_t_r_consE; simp)+
+    apply (erule conjE)+
+    apply (drule_tac t = "type_repr _" in sym)+
+    apply clarsimp
+    apply (frule tprim_no_pointers(1); clarsimp)
+    apply (drule tprim_no_pointers(2); clarsimp)
+    apply (frule tfun_no_pointers(1); clarsimp)
+    apply (frule tfun_no_pointers(2); clarsimp)
+    apply (drule uval_typing_uvalfun; simp)
+    apply (frule tfun_no_pointers(1); clarsimp)
+    apply (frule tfun_no_pointers(2); clarsimp)
+    apply (drule uval_typing_uvalfun; simp)
+    apply (erule u_t_r_emptyE; clarsimp)
+    apply (rename_tac ra wa ro wo)
+    apply (cut_tac \<Xi>' = \<Xi>' and \<sigma> = \<sigma> and v = obsv and \<tau> = \<tau>o and r = ro and w = wo
+        in bang_not_writable(1); simp add: bang\<tau>o)
+    apply (clarsimp simp: crepeat_def valrela val_rel_word val_rel_fun_tag)
+    apply (wp; (clarsimp split: prod.splits)?)
      apply (rule_tac 
-      I = "\<lambda>(a, b, c, j) s. b = c \<and> val_rel obsv (t2_C.obsv_C c) \<and> j \<le> n_C v' \<and>
-            (\<exists>\<sigma>' y. urepeat_bod \<xi>_0 (unat j) (uvalfun_to_expr f) (uvalfun_to_expr g) \<sigma> \<sigma>'
-                    Generated_TypeProof.abbreviatedType1 acc (TPrim (Num U64)) obsv y \<and>
-                   (\<sigma>', s) \<in> state_rel \<and> val_rel y (t2_C.acc_C c))" and
-      M = "\<lambda>((_,_,_, j), _). unat (n_C v') - unat j" in whileLoopE_add_invI)
-     apply (wp; clarsimp split: prod.splits)
-         apply (rename_tac s' prev0 b1 c2 j2 b c1 j1 c j0 bool prev b0 c0 j)
-         apply (wp dispatch_step; clarsimp)
-        apply clarsimp
-        apply (wp; clarsimp)
-       apply clarsimp
-       apply (wp; simp?)
-       apply (wp dispatch_stop; clarsimp)
-     apply clarsimp
-     apply (intro exI conjI; simp?; clarsimp simp: word_less_nat_alt)
-    apply wp
-   apply (rule validNF_select_UNIV)
+      I = "\<lambda>(a, b, j) s. repeat_inv state_rel \<xi>' j fstop fstep \<sigma> \<tau>a \<tau>o acc obsv s (nC v') (a1C b) (o1C b)" and
+      M = "\<lambda>((_,_, j), _). repeat_measure j (nC v')" in whileLoopE_add_invI)
+        apply (wp; clarsimp split: prod.splits)
+            using d1corres o1C_a1U a1C_a1U
+            apply (wp step_wp[OF _ \<xi>'matchesu determ \<tau>fdef fsteptype valrelc]; simp?)
+           apply (wp; clarsimp)
+          apply (wp; clarsimp)
+          using d0corres
+          apply (wp stop_wp[OF _ \<xi>'matchesu determ \<tau>fdef fstoptype fsteptype valrelc]; simp?)
+         apply clarsimp
+         apply (clarsimp simp: repeat_inv_def)
+         apply (intro exI conjI; assumption?)
+          apply (clarsimp simp: unat_mono)
+         apply clarsimp
+        apply (clarsimp simp: repeat_inv_def)
+       apply wp
+      apply (rule validNF_select_UNIV)+
+    apply (clarsimp simp: repeat_inv_def o1C_o1U a1C_o1U a1C_a1U)
+    done
+next
+  show "\<Gamma> ! i = Some (fst (snd (\<Xi>' name)))"
+    using \<Gamma>i by simp
+qed
+
+
+lemma crepeat_corres:
+  assumes \<gamma>len: "i < length \<gamma>"
+  and     valrel: "val_rel (\<gamma> ! i) (v' :: ('a :: cogent_C_val))"
+  and     \<Gamma>i: "\<Gamma> ! i = Some (fst (snd (\<Xi>' name)))"
+  and     \<Xi>name: "\<Xi>' name = ([], \<tau>, \<tau>a)"
+  and     \<tau>def: "\<tau> = TRecord [(''n'', TPrim (Num U64), Present),
+                              (''stop'', TFun (bang \<tau>f) (TPrim Bool), Present),
+                              (''step'', TFun \<tau>f \<tau>a, Present),
+                              (''acc'', \<tau>a, Present), (''obsv'', \<tau>o, Present)] Unboxed"
+  and     \<tau>fdef: "\<tau>f = TRecord [(''acc'', \<tau>a, Present), (''obsv'', \<tau>o, Present)] Unboxed"
+  and     bang\<tau>o: "bang \<tau>o = \<tau>o"
+  and     \<xi>''name: "\<xi>'' name = urepeat \<Xi>' \<xi>' \<tau>a \<tau>o"
+  and     \<xi>'matchesu: "\<xi>' matches-u \<Xi>'"
+  and     determ: "determ \<xi>'"
+  and     \<gamma>i: "\<exists>n acc obsv a b. \<gamma> ! i = URecord [n, (fstop, a), (fstep, b), acc, obsv]"
+  and     fstoptype: "\<Xi>', [], [Some (bang \<tau>f)] \<turnstile> App (uvalfun_to_expr fstop) (Var 0) : TPrim Bool"
+  and     fsteptype: "\<Xi>', [], [Some \<tau>f] \<turnstile> App (uvalfun_to_expr fstep) (Var 0) : \<tau>a"
+  and     d0corres: "\<And>x x' \<sigma> s. val_rel x (x' :: ('c :: cogent_C_val)) \<Longrightarrow>
+                                  corres state_rel (App (uvalfun_to_expr fstop) (Var 0))
+                                    (do ret <- d0 (stopC v') x'; gets (\<lambda>s. ret) od)
+                                    \<xi>' [x] \<Xi>' [option.Some (bang \<tau>f)] \<sigma> s"
+  and     d1corres: "\<And>x x' \<sigma> s. val_rel x x' \<Longrightarrow>
+                                  corres state_rel (App (uvalfun_to_expr fstep) (Var 0))
+                                    (do ret <- d1 (stepC v') x'; gets (\<lambda>s. ret) od)
+                                    \<xi>' [x] \<Xi>' [option.Some \<tau>f] \<sigma> s"
+  and     valrela:  "\<And>x x'. val_rel x (x' :: 'a) \<equiv>
+                              \<exists>n f g acc obsv. x = URecord [n, f, g, acc, obsv] \<and>
+                                val_rel (fst n) (nC x') \<and> val_rel (fst f) (stopC x') \<and>
+                                val_rel (fst g) (stepC x') \<and> val_rel (fst acc) (a0C x') \<and>
+                                val_rel (fst obsv) (o0C x')"
+  and     valrelc:  "\<And>x x'. val_rel x (x' :: 'c) \<equiv>
+                              \<exists>acc obsv. x = URecord [acc, obsv] \<and> val_rel (fst acc) (a1C x') \<and>
+                                val_rel (fst obsv) (o1C x')"
+  and     a1C_a1U: "\<And>x y. a1C (a1U (\<lambda>_. y) x) = y"
+  and     a1C_o1U: "\<And>x y. a1C (o1U y x) = a1C x"
+  and     o1C_o1U: "\<And>x y. o1C (o1U (\<lambda>_. y) x) = y"
+  and     o1C_a1U: "\<And>x y. o1C (a1U y x) = o1C x"
+  and     cfundef: "cfun = crepeat nC stopC stepC a0C o0C a1C a1U o1U d0 d1"
+shows
+  "corres state_rel (App (AFun name []) (Var i))
+    (do x <- cfun v'; gets (\<lambda>s. x) od)
+     \<xi>'' \<gamma> \<Xi>' \<Gamma> \<sigma> s"
+  apply (insert \<gamma>i valrel; clarsimp simp: valrela val_rel_word corres_def)
+  apply (frule matches_ptrs_length)
+  apply (frule_tac  matches_ptrs_proj_single'[OF _ _ \<Gamma>i[simplified \<Xi>name \<tau>def]]; simp?)
+   apply (cut_tac \<gamma>len; linarith)
   apply clarsimp
-  done
-(* 
-lemma dispatch_step:
-  "\<And>v' \<sigma> f g acc ra wa obsv ro b c j0 j.
-    \<lbrakk>proc_ctx_wellformed \<Xi>; val_rel g FUN_ENUM_log2step;
-     upd.uval_typing \<Xi> \<sigma> acc Generated_TypeProof.abbreviatedType1 ra wa; wa \<inter> ro = {};
-     upd.uval_typing \<Xi> \<sigma> obsv (TPrim (Num U64)) ro {}\<rbrakk> \<Longrightarrow>
-    \<lbrace>\<lambda>sa. j = j0 \<and>
-          b = c \<and> val_rel obsv (t2_C.obsv_C c) \<and> j < n_C v' \<and>
-          (\<exists>\<sigma>' y. repeat_bod \<xi>_0 (unat j) (uvalfun_to_expr f) (uvalfun_to_expr g) \<sigma> \<sigma>'
-              Generated_TypeProof.abbreviatedType1 acc (TPrim (Num U64)) obsv y \<and>
-            (\<sigma>', sa) \<in> state_rel \<and> val_rel y (t2_C.acc_C c) \<and>
-            (\<xi>_0, [URecord [(y, type_repr (bang Generated_TypeProof.abbreviatedType1)), (obsv, RPrim (Num U64))]]
-                \<turnstile> (\<sigma>', App (uvalfun_to_expr f) (Var 0)) \<Down>! (\<sigma>', UPrim (LBool False))) \<and>
-            \<not>(\<xi>_0, [URecord [(y, type_repr (bang Generated_TypeProof.abbreviatedType1)), (obsv, RPrim (Num U64))]]
-                \<turnstile> (\<sigma>', App (uvalfun_to_expr f) (Var 0)) \<Down>! (\<sigma>', UPrim (LBool True))))\<rbrace>
-      dispatch_t4' FUN_ENUM_log2step c 
-    \<lbrace>\<lambda>y' sb. t2_C.acc_C_update (\<lambda>_. y') b = t2_C.acc_C_update (\<lambda>_. y') c \<and>
-            val_rel obsv (t2_C.obsv_C c) \<and>
-            j0 + 1 \<le> n_C v' \<and>
-            (\<exists>\<sigma>' y.
-              repeat_bod \<xi>_0 (unat (j0 + 1)) (uvalfun_to_expr f) (uvalfun_to_expr g) \<sigma> \<sigma>'
-                Generated_TypeProof.abbreviatedType1 acc (TPrim (Num U64)) obsv y \<and>
-              (\<sigma>', sb) \<in> state_rel \<and> val_rel y y') \<and>
-            unat (n_C v') - unat (j0 + 1) < unat (n_C v') - unat j\<rbrace>!"
-  unfolding dispatch_t4'_def[simplified unknown_bind_ignore]
-  apply simp
-  apply (clarsimp simp: validNF_def valid_def no_fail_def)
-  apply (subst all_imp_conj_distrib[symmetric]; clarsimp)
-  apply (rename_tac s \<sigma>' y)
-  apply (cut_tac \<sigma> = \<sigma>' and s = s and a' = c and
-      a = "URecord [(y, type_repr Generated_TypeProof.abbreviatedType1),
-            (obsv, type_repr (TPrim (Num U64)))]" in corres_log2step[simplified \<Xi>_def[symmetric]])
-   apply (clarsimp simp: val_rel_simp)
+  apply (erule u_t_recE; clarsimp)
+  apply (erule u_t_r_consE; simp)+
+  apply (erule u_t_r_emptyE; simp)
+  apply (elim conjE)
+  apply (drule_tac t = "type_repr _" in sym)
+  apply clarsimp
+  apply (thin_tac "_ \<inter> _ = {}")+
+  apply (thin_tac "_ \<subseteq> _")+
+  apply (thin_tac "_, _ \<turnstile> _ :u _ \<langle>_, _\<rangle>")+
+  apply (cut_tac state_rel = state_rel and \<sigma> = \<sigma> and s = s and \<xi>'' = \<xi>'' in 
+      crepeat_corres_base[OF \<gamma>len valrel _ _ \<tau>def \<tau>fdef bang\<tau>o _ \<xi>'matchesu determ _ fstoptype
+                            fsteptype _ _ valrela valrelc a1C_a1U _ _ _ cfundef]; simp?)
+  using \<Gamma>i apply simp
+  using \<Xi>name apply simp
+  using \<xi>''name apply simp
+  using d0corres apply simp
+  using d1corres apply simp
+  using a1C_o1U apply simp
+  using o1C_o1U apply simp
+  using o1C_a1U apply simp
   apply (clarsimp simp: corres_def)
-  apply (erule impE, rule \<xi>_0_matchesu_\<Xi>)
-  apply (frule_tac \<xi>' = \<xi>_0  and ro = ro and ra = ra and wa = wa and obsv = obsv and acc = acc
-      in repeat_bod_preservation; simp?)
-     apply (rule \<xi>_0_matchesu_\<Xi>)
-    apply blast
-   apply (clarsimp simp: val_rel_fun_tag cogent_function_val_rel untyped_func_enum_defs)
-   apply (intro conjI typing_mono_app_cogent_fun; clarsimp simp: abbreviated_type_defs)
-   apply (rule log2step_typecorrect'[simplified snd_conv fst_conv log2step_type_def abbreviated_type_defs])
-  apply clarsimp
-  apply (rename_tac r' w')
-(*
-  apply (cut_tac \<Xi> = \<Xi> and \<sigma> = \<sigma>' and r = "r' \<union> ro" and w = w' and
-      vs = "[y, obsv]" and
-      ns = "[''acc'', ''obsv'']" and
-      ts = "[Generated_TypeProof.abbreviatedType1, TPrim (Num U64)]" in upd.uval_typing_all_record; simp?)
-   apply (intro upd.u_t_all_cons[where xs= "[_]" and ts = "[_]" and w' = "{}", simplified]
-      upd.u_t_all_cons[where xs= "[]" and ts = "[]" and w' = "{}" and r' = "{}", simplified]
-      upd.u_t_all_empty; simp?)
-    apply (drule_tac u = obsv in upd.uval_typing_frame(1); simp?)
-    apply blast
-   apply (drule_tac v = obsv in upd.frame_noalias_uval_typing'(2); simp?)
-    apply blast
-   apply blast
-*)
-  apply (erule impE)
-   apply (rule_tac x = "r' \<union> ro" in exI)
-   apply (rule_tac x = w' in exI)
-   apply (simp add: log2step_type_def abbreviated_type_defs)
-   apply (intro upd.matches_ptrs_some[where r' = "{}" and w' = "{}", simplified]
-      upd.matches_ptrs_empty[where \<tau>s = "[]", simplified]
-      upd.u_t_struct
-      upd.u_t_r_cons1[where w' = "{}", simplified]
-      upd.u_t_r_cons1[where r' = "{}" and w' = "{}", simplified]
-      upd.u_t_r_empty; simp?)
-    apply (drule_tac u = obsv in upd.uval_typing_frame(1); simp?)
-    apply blast
-   apply (drule_tac v = obsv in upd.frame_noalias_uval_typing'(2); simp?)
-    apply blast
-   apply blast
-  apply clarsimp
-  apply (rename_tac res s')
-  apply (erule_tac x = res in allE)
-  apply (erule_tac x = s' in allE)
-  apply clarsimp
-  apply (rule conjI)
-   apply unat_arith
-  apply (simp only: less_is_non_zero_p1[THEN  unatSuc2])
-  apply (rule conjI)
-   apply (intro exI conjI; assumption?)
-   apply (rule repeat_bod_step; simp?)
-   apply (simp add: val_rel_fun_tag cogent_function_val_rel untyped_func_enum_defs)
-   apply (rule u_sem_app[where ts ="[]" and y = "Var 0" and \<gamma> = "[_]",
-        simplified,OF _ u_sem_var, simplified]; simp?)
-   apply (intro u_sem_fun)
-  apply unat_arith
   done
 
-inductive_cases u_sem_appE: "\<xi>',\<gamma> \<turnstile> (\<sigma>,App x y)\<Down>! (\<sigma>',v)"
-inductive_cases u_sem_funE: "\<xi>',\<gamma> \<turnstile> (\<sigma>,Fun x y)\<Down>! (\<sigma>',v)"
-inductive_cases u_sem_afunE: "\<xi>',\<gamma> \<turnstile> (\<sigma>,AFun x y)\<Down>! (\<sigma>',v)"
-inductive_cases u_sem_primE: "\<xi>',\<gamma> \<turnstile> (\<sigma>,Prim x y)\<Down>! (\<sigma>',v)"
-inductive_cases u_sem_consE: "\<xi>',\<gamma> \<turnstile>* (\<sigma>,xs)\<Down>! (\<sigma>',v)"
-
-lemma log2stop_deterministic:
-  "\<lbrakk>\<xi>_0, [URecord [(a, f), (b, g)]] \<turnstile> (\<sigma>, Generated_TypeProof.log2stop) \<Down>! (\<sigma>', c); d \<noteq> c\<rbrakk>
-    \<Longrightarrow> \<not>(\<xi>_0, [URecord [(a, f), (b, g)]] \<turnstile> (\<sigma>, App (Fun Generated_TypeProof.log2stop []) (Var 0)) \<Down>! (\<sigma>'', d))"
-  "\<lbrakk>\<xi>_0, [URecord [(a, f), (b, g)]] \<turnstile> (\<sigma>, Generated_TypeProof.log2stop) \<Down>! (\<sigma>', c); \<sigma>' \<noteq> \<sigma>''\<rbrakk>
-    \<Longrightarrow> \<not>(\<xi>_0, [URecord [(a, f), (b, g)]] \<turnstile> (\<sigma>, App (Fun Generated_TypeProof.log2stop []) (Var 0)) \<Down>! (\<sigma>'', d))"
-  unfolding log2stop_def abbreviatedType1_def
-  apply (fastforce elim: u_sem_takeE u_sem_appE u_sem_funE u_sem_afunE u_sem_primE u_sem_consE)+
-  done
-
-lemma dispatch_stop:
-  "\<And>v' \<sigma> f g acc ra wa obsv ro j b c j'.
-    \<lbrakk>proc_ctx_wellformed \<Xi>; val_rel f FUN_ENUM_log2stop; val_rel g FUN_ENUM_log2step;
-     upd.uval_typing \<Xi> \<sigma> acc Generated_TypeProof.abbreviatedType1 ra wa; wa \<inter> ro = {};
-     upd.uval_typing \<Xi> \<sigma> obsv (TPrim (Num U64)) ro {}\<rbrakk> \<Longrightarrow>
-    \<lbrace>\<lambda>sa. (\<exists>\<sigma>' y n. (\<sigma>', sa) \<in> state_rel \<and> val_rel y (t2_C.acc_C c) \<and> val_rel obsv (t2_C.obsv_C c) \<and>
-            j = j' \<and> b = c \<and> j < n_C v' \<and>
-            repeat_bod \<xi>_0 n (uvalfun_to_expr f) (uvalfun_to_expr g) \<sigma> \<sigma>'
-              Generated_TypeProof.abbreviatedType1 acc (TPrim (Num U64)) obsv y \<and>
-            ((\<xi>_0 , [URecord [(y, type_repr (bang Generated_TypeProof.abbreviatedType1)),
-                (obsv, type_repr (TPrim (Num U64)))]]
-                \<turnstile> (\<sigma>', App (uvalfun_to_expr f) (Var 0)) \<Down>! (\<sigma>', UPrim (LBool True))) \<and>
-             \<not>(\<xi>_0 , [URecord [(y, type_repr (bang Generated_TypeProof.abbreviatedType1)),
-                (obsv, type_repr (TPrim (Num U64)))]]
-                \<turnstile> (\<sigma>', App (uvalfun_to_expr f) (Var 0)) \<Down>! (\<sigma>', UPrim (LBool False)))
-              \<longrightarrow> n \<ge> unat j \<and> n < unat (n_C v')) \<and>
-            ((\<xi>_0 , [URecord [(y, type_repr (bang Generated_TypeProof.abbreviatedType1)),
-                (obsv, type_repr (TPrim (Num U64)))]]
-                \<turnstile> (\<sigma>', App (uvalfun_to_expr f) (Var 0)) \<Down>! (\<sigma>', UPrim (LBool False))) \<and>
-             \<not>(\<xi>_0 , [URecord [(y, type_repr (bang Generated_TypeProof.abbreviatedType1)),
-                (obsv, type_repr (TPrim (Num U64)))]]
-                \<turnstile> (\<sigma>', App (uvalfun_to_expr f) (Var 0)) \<Down>! (\<sigma>', UPrim (LBool True)))
-              \<longrightarrow> n = unat j))\<rbrace>
-      dispatch_t3' FUN_ENUM_log2stop b 
-    \<lbrace>\<lambda>x sb.
-        (boolean_C x \<noteq> 0 \<longrightarrow>
-            (\<exists>\<sigma>' y.
-              repeat_bod \<xi>_0 (unat (n_C v')) (uvalfun_to_expr f) (uvalfun_to_expr g) \<sigma> \<sigma>'
-                Generated_TypeProof.abbreviatedType1 acc (TPrim (Num U64)) obsv y \<and>
-              (\<sigma>', sb) \<in> state_rel \<and> val_rel y (t2_C.acc_C c))) \<and>
-        (boolean_C x = 0 \<longrightarrow>
-            j = j' \<and>
-            b = c \<and>
-            val_rel obsv (t2_C.obsv_C c) \<and>
-            j < n_C v' \<and>
-            (\<exists>\<sigma>' y.
-              repeat_bod \<xi>_0 (unat j) (uvalfun_to_expr f) (uvalfun_to_expr g) \<sigma> \<sigma>'
-                Generated_TypeProof.abbreviatedType1 acc (TPrim (Num U64)) obsv y \<and>
-              (\<sigma>', sb) \<in> state_rel \<and> val_rel y (t2_C.acc_C c) \<and>
-               (\<xi>_0, [URecord [(y, type_repr (bang Generated_TypeProof.abbreviatedType1)), (obsv, RPrim (Num U64))]]
-                \<turnstile> (\<sigma>', App (uvalfun_to_expr f) (Var 0)) \<Down>! (\<sigma>', UPrim (LBool False))) \<and>
-              \<not>(\<xi>_0, [URecord [(y, type_repr (bang Generated_TypeProof.abbreviatedType1)), (obsv, RPrim (Num U64))]]
-                \<turnstile> (\<sigma>', App (uvalfun_to_expr f) (Var 0)) \<Down>! (\<sigma>', UPrim (LBool True)))))\<rbrace>!"
-  unfolding dispatch_t3'_def[simplified unknown_bind_ignore]
-  apply simp
-  apply (clarsimp simp: validNF_def valid_def no_fail_def)
-  apply (subst all_imp_conj_distrib[symmetric]; clarsimp)
-  apply (rename_tac s \<sigma>' y n)
-  apply (cut_tac \<sigma> = \<sigma>' and s = s and a' = c and
-      a = "URecord [(y, type_repr Generated_TypeProof.abbreviatedType1),
-            (obsv, type_repr (TPrim (Num U64)))]" in corres_log2stop[simplified \<Xi>_def[symmetric]])
-   apply (clarsimp simp: val_rel_simp)
+lemma crepeat_corres_rel_leq:
+  assumes \<gamma>len: "i < length \<gamma>"
+  and     valrel: "val_rel (\<gamma> ! i) (v' :: ('a :: cogent_C_val))"
+  and     \<Gamma>i: "\<Gamma> ! i = Some (fst (snd (\<Xi>' name)))"
+  and     \<Xi>name: "\<Xi>' name = ([], \<tau>, \<tau>a)"
+  and     \<tau>def: "\<tau> = TRecord [(''n'', TPrim (Num U64), Present),
+                              (''stop'', TFun (bang \<tau>f) (TPrim Bool), Present),
+                              (''step'', TFun \<tau>f \<tau>a, Present),
+                              (''acc'', \<tau>a, Present), (''obsv'', \<tau>o, Present)] Unboxed"
+  and     \<tau>fdef: "\<tau>f = TRecord [(''acc'', \<tau>a, Present), (''obsv'', \<tau>o, Present)] Unboxed"
+  and     bang\<tau>o: "bang \<tau>o = \<tau>o"
+  and     \<xi>''name: "\<xi>'' name = urepeat \<Xi>' \<xi>' \<tau>a \<tau>o"
+  and     leq: "rel_leq \<xi>' \<xi>''"
+  and     determ: "determ \<xi>''"
+  and     \<gamma>i: "\<exists>n acc obsv a b. \<gamma> ! i = URecord [n, (fstop, a), (fstep, b), acc, obsv]"
+  and     fstoptype: "\<Xi>', [], [Some (bang \<tau>f)] \<turnstile> App (uvalfun_to_expr fstop) (Var 0) : TPrim Bool"
+  and     fsteptype: "\<Xi>', [], [Some \<tau>f] \<turnstile> App (uvalfun_to_expr fstep) (Var 0) : \<tau>a"
+  and     d0corres: "\<And>x x' \<sigma> s. val_rel x (x' :: ('c :: cogent_C_val)) \<Longrightarrow>
+                                  corres state_rel (App (uvalfun_to_expr fstop) (Var 0))
+                                    (do ret <- d0 (stopC v') x'; gets (\<lambda>s. ret) od)
+                                    \<xi>' [x] \<Xi>' [option.Some (bang \<tau>f)] \<sigma> s"
+  and     d1corres: "\<And>x x' \<sigma> s. val_rel x x' \<Longrightarrow>
+                                  corres state_rel (App (uvalfun_to_expr fstep) (Var 0))
+                                    (do ret <- d1 (stepC v') x'; gets (\<lambda>s. ret) od)
+                                    \<xi>' [x] \<Xi>' [option.Some \<tau>f] \<sigma> s"
+  and     valrela:  "\<And>x x'. val_rel x (x' :: 'a) \<equiv>
+                              \<exists>n f g acc obsv. x = URecord [n, f, g, acc, obsv] \<and>
+                                val_rel (fst n) (nC x') \<and> val_rel (fst f) (stopC x') \<and>
+                                val_rel (fst g) (stepC x') \<and> val_rel (fst acc) (a0C x') \<and>
+                                val_rel (fst obsv) (o0C x')"
+  and     valrelc:  "\<And>x x'. val_rel x (x' :: 'c) \<equiv>
+                              \<exists>acc obsv. x = URecord [acc, obsv] \<and> val_rel (fst acc) (a1C x') \<and>
+                                val_rel (fst obsv) (o1C x')"
+  and     a1C_a1U: "\<And>x y. a1C (a1U (\<lambda>_. y) x) = y"
+  and     a1C_o1U: "\<And>x y. a1C (o1U y x) = a1C x"
+  and     o1C_o1U: "\<And>x y. o1C (o1U (\<lambda>_. y) x) = y"
+  and     o1C_a1U: "\<And>x y. o1C (a1U y x) = o1C x"
+  and     cfundef: "cfun = crepeat nC stopC stepC a0C o0C a1C a1U o1U d0 d1"
+shows
+  "corres state_rel (App (AFun name []) (Var i))
+    (do x <- cfun v'; gets (\<lambda>s. x) od)
+     \<xi>'' \<gamma> \<Xi>' \<Gamma> \<sigma> s"
   apply (clarsimp simp: corres_def)
-  apply (erule impE, rule \<xi>_0_matchesu_\<Xi>)
- apply (frule_tac \<xi>' = \<xi>_0  and ro = ro and ra = ra and wa = wa and obsv = obsv and acc = acc
-      in repeat_bod_preservation; simp?)
-     apply (rule \<xi>_0_matchesu_\<Xi>)
-    apply blast
-   apply (clarsimp simp: val_rel_fun_tag cogent_function_val_rel untyped_func_enum_defs)
-   apply (intro conjI typing_mono_app_cogent_fun; clarsimp simp: abbreviated_type_defs)
-   apply (rule log2step_typecorrect'[simplified snd_conv fst_conv log2step_type_def abbreviated_type_defs])
-  apply clarsimp
-  apply (rename_tac r' w')
-  apply (erule impE, rule_tac x = "r' \<union> ro" in exI)
-   apply (rule_tac x = w' in exI)
-  apply (simp add: log2stop_type_def abbreviated_type_defs)
-   apply (intro upd.matches_ptrs_some[where r' = "{}" and w' = "{}", simplified]
-      upd.matches_ptrs_empty[where \<tau>s = "[]", simplified]
-      upd.u_t_struct
-      upd.u_t_r_cons1[where w' = "{}", simplified]
-      upd.u_t_r_cons1[where r' = "{}" and w' = "{}", simplified]
-      upd.u_t_r_empty; simp?)
-    apply (drule_tac u = obsv in upd.uval_typing_frame(1); simp?)
-    apply blast
-   apply (drule_tac v = obsv in upd.frame_noalias_uval_typing'(2); simp?)
-    apply blast
-   apply blast
-  apply clarsimp
-  apply (rename_tac res s')
-  apply (erule_tac x = res in allE)
-  apply (erule_tac x = s' in allE)
-  apply clarsimp 
-  apply (drule_tac w = "{}" and r = "(r' \<union> w') \<union> ro" and \<tau> = "TPrim Bool" and
-      ?\<Gamma>.0 = "[option.Some Generated_TypeProof.abbreviatedType2]"
-      in upd.preservation_mono(1)[OF _ _  \<xi>_0_matchesu_\<Xi>]; simp?)
-    apply (drule_tac v = y in upd.uval_typing_bang(1))
-    apply (clarsimp simp: abbreviated_type_defs)
-    apply (intro upd.matches_ptrs_some[where r' = "{}" and w' = "{}", simplified]
-      upd.matches_ptrs_empty[where \<tau>s = "[]", simplified]
-      upd.u_t_struct
-      upd.u_t_r_cons1[where w' = "{}", simplified]
-      upd.u_t_r_cons1[where r' = "{}" and w' = "{}", simplified]
-      upd.u_t_r_empty; simp?)
-    apply (drule_tac u = obsv in upd.uval_typing_frame(1); simp?)
-    apply blast
-   apply (drule_tac v = obsv in upd.frame_noalias_uval_typing'(2); simp?)
-    apply blast
-   apply (rule log2stop_typecorrect'[simplified fst_conv snd_conv log2stop_type_def])
-  apply clarsimp
-  apply (frule_tac v = r in upd.tprim_no_pointers(1))
-  apply (drule_tac v = r in upd.tprim_no_pointers(2))
-  apply clarsimp
-  apply (drule upd.frame_empty; clarsimp)
-  apply (rule conjI; clarsimp simp: val_rel_bool_t_C_def)
-  apply (erule impE)
-    apply (clarsimp simp: val_rel_fun_tag cogent_function_val_rel untyped_func_enum_defs abbreviated_type_defs)
-    apply (rule conjI)
-     apply (rule u_sem_app[where ts ="[]" and y = "Var 0" and \<gamma> = "[_]",
-        simplified,OF _ u_sem_var, simplified]; simp?)
-     apply (intro u_sem_fun)
-    apply (drule_tac d = "UPrim (LBool False)" and \<sigma>'' = \<sigma>'' in log2stop_deterministic(1);simp)
-   apply (intro exI conjI; simp?)
-   apply (rule_tac i = n in repeat_bod_early_termination; simp add: word_less_nat_alt)
-   apply (clarsimp simp: val_rel_fun_tag cogent_function_val_rel untyped_func_enum_defs abbreviated_type_defs)
-   apply (rule u_sem_app[where ts ="[]" and y = "Var 0" and \<gamma> = "[_]",
-        simplified,OF _ u_sem_var, simplified]; simp?)
-    apply (intro u_sem_fun)
-   apply (clarsimp simp: val_rel_fun_tag cogent_function_val_rel untyped_func_enum_defs abbreviated_type_defs)
-   apply (drule_tac d = "UPrim (LBool False)" and \<sigma>'' = \<sigma>'' in log2stop_deterministic(1);simp)
-  apply (thin_tac "_ \<longrightarrow> _")
-  apply (clarsimp simp: val_rel_fun_tag cogent_function_val_rel untyped_func_enum_defs abbreviated_type_defs)
-  apply (frule_tac d = "UPrim (LBool True)" and \<sigma>'' = \<sigma>'' in log2stop_deterministic(1);simp)
-  apply (erule impE)
-   apply (rule u_sem_app[where ts ="[]" and y = "Var 0" and \<gamma> = "[_]",
-        simplified,OF _ u_sem_var, simplified]; simp?)
-   apply (intro u_sem_fun)
-  apply (intro exI conjI; simp)
-  apply (rule u_sem_app[where ts ="[]" and y = "Var 0" and \<gamma> = "[_]",
-        simplified,OF _ u_sem_var, simplified]; simp?)
-  apply (intro u_sem_fun)
+  apply (cut_tac state_rel = state_rel and \<sigma> = \<sigma> and s = s and \<xi>'' = \<xi>'' in 
+      crepeat_corres[OF \<gamma>len valrel _ _ \<tau>def \<tau>fdef bang\<tau>o _ rel_leq_matchesuD[OF leq]
+                       determ_rel_leqD[OF leq determ] \<gamma>i fstoptype fsteptype _ _ valrela
+                       valrelc a1C_a1U _ _ _ cfundef]; simp?)
+  using \<Gamma>i apply simp
+  using \<Xi>name apply simp
+  using \<xi>''name apply simp
+  using d0corres apply simp
+  using d1corres apply simp
+  using a1C_o1U apply simp
+  using o1C_o1U apply simp
+  using o1C_a1U apply simp
+  apply (clarsimp simp: corres_def)
   done
 
-lemma 
-  "\<And>v' i \<gamma> \<Gamma> \<sigma> s.
-    \<lbrakk>stop_C v' = FUN_ENUM_log2stop; step_C v' = FUN_ENUM_log2step; i < length \<gamma>; val_rel (\<gamma> ! i) v';
-     \<Gamma> ! i = Some (fst (snd repeat_0_type))\<rbrakk>
-    \<Longrightarrow> corres state_rel (App (AFun ''repeat_0'' []) (Var i)) (do x <- repeat_0' v';
- gets (\<lambda>s. x)
-                                                               od)
-         \<xi>_1 \<gamma> \<Xi> \<Gamma> \<sigma> s"
-  apply (rule absfun_corres; simp?)
-   prefer 2
-  \<comment>\<open>For automation, make a repeat_type_defs lemma\<close>
-   apply (clarsimp simp: repeat_0_type_def abbreviated_type_defs \<Xi>_def)
-  apply (subst abs_fun_rel_def'; clarsimp)
-  apply (rotate_tac -1)
-  apply (subst (asm) \<Xi>_def; clarsimp)
-  apply (clarsimp simp: repeat_0_type_def)
-  apply (subst (asm) val_rel_simp; clarsimp)
-  apply (rename_tac r w n rn f rf g rg acc racc obsv robsv)
-  apply (subst (asm) val_rel_word64; clarsimp)
-  apply (erule upd.u_t_recE; clarsimp)
-  apply (erule upd.u_t_r_consE; clarsimp)+
-  apply (erule upd.u_t_r_emptyE; clarsimp)
-  apply (frule upd.tprim_no_pointers(1); clarsimp)
-  apply (frule upd.tprim_no_pointers(2); clarsimp)
-  apply (frule upd.tfun_no_pointers(1); clarsimp)
-  apply (drule upd.tfun_no_pointers(2); clarsimp)
-  apply (frule upd.tfun_no_pointers(1); clarsimp)
-  apply (drule upd.tfun_no_pointers(2); clarsimp)
-  apply (rename_tac f g acc ra wa obsv ro wo)
-  apply (frule_tac v = obsv and K' = "[]" in upd.discardable_or_shareable_not_writable'(1)[rotated 2]; simp?)
-    apply (rule kindingI; simp)
-   apply blast
-  apply clarsimp
-  unfolding repeat_0'_def
-  apply (clarsimp simp: L2polish unknown_bind_ignore)
-  apply (subst \<xi>1_def; clarsimp simp: repeat_def)
-  apply (subgoal_tac "is_uvalfun f \<and>
-               is_uvalfun g \<and>
-               \<Xi>, [], [Some (TRecord
-                               [(''acc'', bang Generated_TypeProof.abbreviatedType1, Present),
-                                (''obsv'', TPrim (Num U64), Present)]
-                               Unboxed)] \<turnstile> App (uvalfun_to_expr f) (Var 0) : TPrim Bool \<and>
-               \<Xi>, [], [Some (TRecord
-                               [(''acc'', Generated_TypeProof.abbreviatedType1, Present), (''obsv'', TPrim (Num U64), Present)]
-                               Unboxed)] \<turnstile> App (uvalfun_to_expr g) (Var 0) : Generated_TypeProof.abbreviatedType1")
-   apply simp
-   apply (thin_tac "_ \<and> _ \<and> _ \<and> _")
-   defer
-   apply (clarsimp simp: val_rel_simp cogent_function_val_rel untyped_func_enum_defs)
-   apply (intro conjI typing_mono_app_cogent_fun; clarsimp simp: abbreviated_type_defs)
-    apply (rule log2stop_typecorrect'[simplified snd_conv fst_conv log2stop_type_def abbreviated_type_defs])
-   apply (rule log2step_typecorrect'[simplified snd_conv fst_conv log2step_type_def abbreviated_type_defs])
-  apply (wp; (clarsimp split: prod.splits)?)
-     apply (rename_tac breakval)
-     apply (rule_tac 
-      I = "\<lambda>(a, b, c, j) s. b = c \<and> val_rel obsv (t2_C.obsv_C c) \<and> j \<le> n_C v' \<and>
-            (\<exists>\<sigma>' y. repeat_bod \<xi>_0 (unat j) (uvalfun_to_expr f) (uvalfun_to_expr g) \<sigma> \<sigma>'
-                    Generated_TypeProof.abbreviatedType1 acc (TPrim (Num U64)) obsv y \<and>
-                   (\<sigma>', s) \<in> state_rel \<and> val_rel y (t2_C.acc_C c))" and
-      M = "\<lambda>((_,_,_, j), _). unat (n_C v') - unat j" in whileLoopE_add_invI)
-     apply (wp; clarsimp split: prod.splits)
-         apply (rename_tac s' prev0 b1 c2 j2 b c1 j1 c j0 bool prev b0 c0 j)
-         apply (wp dispatch_step; clarsimp)
-        apply clarsimp
-        apply (wp; clarsimp)
-       apply clarsimp
-       apply (wp; simp?)
-       apply (wp dispatch_stop; clarsimp)
-     apply clarsimp
-     apply (intro exI conjI; simp?; clarsimp simp: word_less_nat_alt)
-    apply wp
-   apply (rule validNF_select_UNIV)
-  apply clarsimp
+
+lemma crepeat_corres_bang:
+  assumes \<gamma>len: "i < length \<gamma>"
+  and     valrel: "val_rel (\<gamma> ! i) (v' :: ('a :: cogent_C_val))"
+  and     \<Gamma>i: "\<Gamma> ! i = Some (fst (snd (\<Xi>' name)))"
+  and     \<Xi>name: "\<Xi>' name = ([], \<tau>, \<tau>a)"
+  and     \<tau>def: "\<tau> = TRecord [(''n'', TPrim (Num U64), Present),
+                              (''stop'', TFun \<tau>f (TPrim Bool), Present),
+                              (''step'', TFun \<tau>f \<tau>a, Present),
+                              (''acc'', \<tau>a, Present), (''obsv'', \<tau>o, Present)] Unboxed"
+  and     \<tau>fdef: "\<tau>f = TRecord [(''acc'', \<tau>a, Present), (''obsv'', \<tau>o, Present)] Unboxed"
+  and     bang\<tau>a: "bang \<tau>a = \<tau>a"
+  and     bang\<tau>o: "bang \<tau>o = \<tau>o"
+  and     \<xi>''name: "\<xi>'' name = urepeat \<Xi>' \<xi>' \<tau>a \<tau>o"
+  and     leq: "rel_leq \<xi>' \<xi>''"
+  and     determ: "determ \<xi>''"
+  and     \<gamma>i: "\<exists>n acc obsv a b. \<gamma> ! i = URecord [n, (fstop, a), (fstep, b), acc, obsv]"
+  and     fstoptype: "\<Xi>', [], [Some \<tau>f] \<turnstile> App (uvalfun_to_expr fstop) (Var 0) : TPrim Bool"
+  and     fsteptype: "\<Xi>', [], [Some \<tau>f] \<turnstile> App (uvalfun_to_expr fstep) (Var 0) : \<tau>a"
+  and     d0corres: "\<And>x x' \<sigma> s. val_rel x (x' :: ('c :: cogent_C_val)) \<Longrightarrow>
+                                  corres state_rel (App (uvalfun_to_expr fstop) (Var 0))
+                                    (do ret <- d0 (stopC v') x'; gets (\<lambda>s. ret) od)
+                                    \<xi>' [x] \<Xi>' [option.Some (bang \<tau>f)] \<sigma> s"
+  and     d1corres: "\<And>x x' \<sigma> s. val_rel x x' \<Longrightarrow>
+                                  corres state_rel (App (uvalfun_to_expr fstep) (Var 0))
+                                    (do ret <- d1 (stepC v') x'; gets (\<lambda>s. ret) od)
+                                    \<xi>' [x] \<Xi>' [option.Some \<tau>f] \<sigma> s"
+  and     valrela:  "\<And>x x'. val_rel x (x' :: 'a) \<equiv>
+                              \<exists>n f g acc obsv. x = URecord [n, f, g, acc, obsv] \<and>
+                                val_rel (fst n) (nC x') \<and> val_rel (fst f) (stopC x') \<and>
+                                val_rel (fst g) (stepC x') \<and> val_rel (fst acc) (a0C x') \<and>
+                                val_rel (fst obsv) (o0C x')"
+  and     valrelc:  "\<And>x x'. val_rel x (x' :: 'c) \<equiv>
+                              \<exists>acc obsv. x = URecord [acc, obsv] \<and> val_rel (fst acc) (a1C x') \<and>
+                                val_rel (fst obsv) (o1C x')"
+  and     a1C_a1U: "\<And>x y. a1C (a1U (\<lambda>_. y) x) = y"
+  and     a1C_o1U: "\<And>x y. a1C (o1U y x) = a1C x"
+  and     o1C_o1U: "\<And>x y. o1C (o1U (\<lambda>_. y) x) = y"
+  and     o1C_a1U: "\<And>x y. o1C (a1U y x) = o1C x"
+  and     cfundef: "cfun = crepeat nC stopC stepC a0C o0C a1C a1U o1U d0 d1"
+shows
+  "corres state_rel (App (AFun name []) (Var i))
+    (do x <- cfun v'; gets (\<lambda>s. x) od)
+     \<xi>'' \<gamma> \<Xi>' \<Gamma> \<sigma> s"
+  apply (rule_tac state_rel = state_rel and \<sigma> = \<sigma> and s = s in 
+      crepeat_corres_rel_leq[OF \<gamma>len valrel _ _  _  \<tau>fdef bang\<tau>o _ leq
+                       determ \<gamma>i _  fsteptype _ _ valrela
+                       valrelc a1C_a1U _ _ _ cfundef]; simp?)
+  using \<Gamma>i apply simp
+  using \<Xi>name \<tau>def \<tau>fdef bang\<tau>a bang\<tau>o apply simp
+  using \<xi>''name apply simp
+  using \<tau>fdef bang\<tau>a bang\<tau>o fstoptype apply simp
+  using d0corres apply simp
+  using d1corres apply simp
+  using a1C_o1U apply simp
+  using o1C_o1U apply simp
+  using o1C_a1U apply simp
   done
-*)
+
+lemmas crepeat_corres_bang_fun_fun = crepeat_corres_bang
+  [where fstop = "UFunction _ _" and fstep = "UFunction _ _", simplified,
+   OF _ _ _ _ _ _ _ _ _ _ _ _ typing_mono_app_cogent_fun typing_mono_app_cogent_fun]
+lemmas crepeat_corres_bang_fun_afun = crepeat_corres_bang
+  [where fstop = "UFunction _ _" and fstep = "UAFunction _ _", simplified,
+   OF _ _ _ _ _ _ _ _ _ _ _ _ typing_mono_app_cogent_fun typing_mono_app_cogent_absfun]
+lemmas crepeat_corres_bang_afun_fun = crepeat_corres_bang
+  [where fstop = "UAFunction _ _" and fstep = "UFunction _ _", simplified,
+   OF _ _ _ _ _ _ _ _ _ _ _ _ typing_mono_app_cogent_absfun typing_mono_app_cogent_fun]
+lemmas crepeat_corres_bang_afun_afun = crepeat_corres_bang
+  [where fstop = "UAFunction _ _" and fstep = "UAFunction _ _", simplified,
+   OF _ _ _ _ _ _ _ _ _ _ _ _ typing_mono_app_cogent_absfun typing_mono_app_cogent_absfun]
+
+lemmas crepeat_corres_fun_fun = crepeat_corres_rel_leq
+  [where fstop = "UFunction _ _" and fstep = "UFunction _ _", simplified,
+   OF _ _ _ _ _ _ _ _ _ _ _  typing_mono_app_cogent_fun typing_mono_app_cogent_fun]
+lemmas crepeat_corres_fun_afun = crepeat_corres_rel_leq
+  [where fstop = "UFunction _ _" and fstep = "UAFunction _ _", simplified,
+   OF _ _ _ _ _ _ _ _ _ _ _ typing_mono_app_cogent_fun typing_mono_app_cogent_absfun]
+lemmas crepeat_corres_afun_fun = crepeat_corres_rel_leq
+  [where fstop = "UAFunction _ _" and fstep = "UFunction _ _", simplified,
+   OF _ _ _ _ _ _ _ _ _ _ _ typing_mono_app_cogent_absfun typing_mono_app_cogent_fun]
+lemmas crepeat_corres_afun_afun = crepeat_corres_rel_leq
+  [where fstop = "UAFunction _ _" and fstep = "UAFunction _ _", simplified,
+   OF _ _ _ _ _ _ _ _ _ _ _ typing_mono_app_cogent_absfun typing_mono_app_cogent_absfun]
+
 end (* of context *)
+
 end
