cogent/examples/repeat/RepeatAssm.thy
@@ -3,6 +3,7 @@ theory RepeatAssm
     RepeatUpdate
     RepeatValue
     RepeatMono
+    RepeatCorres
     RepeatCorrespondence
     RepeatScorres
     "build/Generated_AllRefine"
@@ -50,7 +51,7 @@ lemma \<xi>_1_matchesu_\<Xi>:
    apply clarsimp
    apply (subst (asm) \<Xi>_def; clarsimp)
    apply (clarsimp simp: repeat_0_type_def)
-   apply (rule urepeat_preservation[OF proc_ctx_wellformed_\<Xi> \<xi>_0_matchesu_\<Xi>]; (simp add: abbreviated_type_defs)?)
+   apply (rule_tac v= v in  urepeat_preservation[OF proc_ctx_wellformed_\<Xi> \<xi>_0_matchesu_\<Xi>]; (simp add: abbreviated_type_defs)?)
   apply (clarsimp simp: \<xi>0_def)
   done
 end (* of context *)
@@ -58,9 +59,26 @@ end (* of context *)
 subsection "Partial ordering on abstract functions"
 
 lemma \<xi>_0_le_\<xi>_1:
-  "\<xi>ule \<xi>_0 \<xi>_1"
-  unfolding \<xi>0_def \<xi>ule_def
+  "rel_leq \<xi>_0 \<xi>_1"
+  unfolding \<xi>0_def rel_leq_def
   by simp
+
+subsection "Abstract functions are deterministic"
+
+lemma \<xi>_0_determ:
+  "determ \<xi>_0"
+  unfolding determ_def \<xi>0_def
+  by simp
+
+lemma \<xi>_1_determ:
+  "determ \<xi>_1"
+  unfolding determ_def \<xi>1_def
+  apply clarsimp
+  apply (rule conjI; clarsimp)
+   apply (drule (1) urepeat_deterministic[OF \<xi>_0_determ]; simp)
+  apply (drule (1) determD[OF \<xi>_0_determ]; simp)
+  done
+
 
 section "Abstract functions specifications for the monomorphic value semantics"
 
@@ -94,9 +112,25 @@ lemma \<xi>m1_matches_\<Xi>:
 subsection "Partial ordering on abstract functions"
 
 lemma \<xi>m0_le_\<xi>m1:
-  "\<xi>vle \<xi>m0 \<xi>m1"
-  unfolding \<xi>m0_def \<xi>vle_def
+  "rel_leq \<xi>m0 \<xi>m1"
+  unfolding \<xi>m0_def rel_leq_def
   by simp
+
+subsection "Abstract functions are deterministic"
+
+lemma \<xi>m0_determ:
+  "determ \<xi>m0"
+  unfolding determ_def \<xi>m0_def
+  by simp
+
+lemma \<xi>m1_determ:
+  "determ \<xi>m1"
+  unfolding determ_def \<xi>m1_def
+  apply clarsimp
+  apply (rule conjI; clarsimp)
+   apply (drule (1) vrepeat_deterministic[OF \<xi>m0_determ]; simp)
+  apply (drule (1) determD[OF \<xi>m0_determ]; simp)
+  done
 
 end (* of context *)
 
@@ -113,9 +147,78 @@ definition \<xi>p1 :: "funtyp \<Rightarrow> (funtyp, 'c) vval \<Rightarrow> (fun
 subsection "Partial ordering on abstract functions"
 
 lemma \<xi>p0_le_\<xi>p1:
-  "\<xi>vle \<xi>p0 \<xi>p1"
-  unfolding \<xi>p0_def \<xi>vle_def
+  "rel_leq \<xi>p0 \<xi>p1"
+  unfolding \<xi>p0_def rel_leq_def
   by simp
+
+subsection "Abstract functions are deterministic"
+
+lemma \<xi>p0_determ:
+  "determ \<xi>p0"
+  unfolding determ_def \<xi>p0_def
+  by simp
+
+lemma \<xi>p1_determ:
+  "determ \<xi>p1"
+  unfolding determ_def \<xi>p1_def
+  apply clarsimp
+  apply (rule conjI; clarsimp)
+   apply (drule (1) prepeat_deterministic[OF \<xi>p0_determ]; simp)
+  apply (drule (1) determD[OF \<xi>p0_determ]; simp)
+  done
+
+section "Correspondence between abstract functions in the update semantics and C"
+
+context Generated begin
+
+lemma repeat_0'_simp:
+  "repeat_0' = crepeat t5_C.n_C t5_C.stop_C t5_C.step_C t5_C.acc_C t5_C.obsv_C t2_C.acc_C t2_C.acc_C_update t2_C.obsv_C_update dispatch_t3' dispatch_t4'"
+  unfolding crepeat_def[polish] repeat_0'_def[simplified L2polish, polish]
+  apply clarsimp
+  done
+
+lemma \<Xi>_simps:
+  "\<Xi> ''repeat_0'' = repeat_0_type"
+  apply (clarsimp simp: \<Xi>_def)
+  done
+
+lemma \<xi>_1_simps:
+  "\<xi>_1 ''repeat_0'' = urepeat \<Xi> \<xi>_0 abbreviatedType1 (TPrim (Num U64))"
+  apply (clarsimp simp: \<xi>1_def fun_eq_iff)
+  done
+
+lemma repeat_corres:
+  "\<And>v' i \<gamma> \<Gamma> \<sigma> s.
+    \<lbrakk>stop_C v' = FUN_ENUM_log2stop; step_C v' = FUN_ENUM_log2step; i < length \<gamma>; val_rel (\<gamma> ! i) v';
+     \<Gamma> ! i = Some (fst (snd repeat_0_type))\<rbrakk>
+    \<Longrightarrow> corres state_rel (App (AFun ''repeat_0'' []) (Var i)) (do x <- repeat_0' v';
+ gets (\<lambda>s. x)
+                                                               od)
+         \<xi>_1 \<gamma> \<Xi> \<Gamma> \<sigma> s"
+  apply simp
+  apply (subst (asm) \<Xi>_simps[symmetric])
+  apply (cut_tac uv = "\<gamma>!i" and x = v' in val_rel_t5_C_def)
+  apply (rule crepeat_corres_bang_fun_fun[
+      where \<tau>f = abbreviatedType2 and \<tau>a = abbreviatedType1 and \<tau>o = "TPrim (Num U64)" and o1C = t2_C.obsv_C,
+      OF _ _ _ \<Xi>_simps[unfolded repeat_0_type_def]  _ _ _  _  \<xi>_1_simps
+      \<xi>_0_le_\<xi>_1 \<xi>_1_determ _
+      log2stop_typecorrect'[simplified log2stop_type_def fst_conv snd_conv]
+      log2step_typecorrect'[simplified log2step_type_def fst_conv snd_conv]
+      _ _ _ _ _ _ _ _ repeat_0'_simp]; (simp add: abbreviated_type_defs)?)
+      apply (clarsimp simp: cogent_function_val_rel untyped_func_enum_defs val_rel_simp)
+     apply (subst abbreviated_type_defs[symmetric])+
+     apply (rule corres_app_concrete[simplified]; simp?)
+     apply (simp add: dispatch_t3'_def unknown_bind_ignore)
+     apply (erule corres_log2stop[folded \<Xi>_def, simplified fst_conv snd_conv log2stop_type_def])
+    apply (subst abbreviated_type_defs[symmetric])+
+    apply (rule corres_app_concrete[simplified]; simp?)
+    apply (simp add: dispatch_t4'_def unknown_bind_ignore)
+    apply (erule corres_log2step[folded \<Xi>_def, simplified fst_conv snd_conv log2step_type_def])
+   apply (clarsimp simp: val_rel_simp)
+  apply (clarsimp simp: val_rel_simp)
+  done
+
+end (* of context *)
 
 section "Correspondence between abstract functions in the update and value semantics"
 
@@ -166,5 +269,16 @@ lemma (in shallow) scorres_repeat:
   "scorres repeat (AFun ''repeat'' ts) \<gamma> \<xi>p1"
   by (rule repeat_scorres[OF \<xi>p0_le_\<xi>p1]; simp add: \<xi>p1_def fun_eq_iff)
 
+section "All refine"
+
+lemmas (in Generated_cogent_shallow) corres_shallow_C_log2step_concrete = corres_shallow_C_log2step
+  [OF _ val.rename_mono_prog_\<xi>m0_\<xi>p0 _ _ proc_ctx_wellformed_\<Xi> val.\<xi>m0_matches_\<Xi>]
+
+lemmas (in Generated_cogent_shallow) corres_shallow_C_log2stop_concrete = corres_shallow_C_log2stop
+  [OF _ val.rename_mono_prog_\<xi>m0_\<xi>p0 _ _ proc_ctx_wellformed_\<Xi> val.\<xi>m0_matches_\<Xi>]
+
+lemmas (in Generated_cogent_shallow) corres_shallow_C_mylog2_concrete = corres_shallow_C_mylog2
+  [folded \<Xi>_def, OF _ _ val.rename_mono_prog_\<Xi>_\<xi>m1_\<xi>p1 _ _ proc_ctx_wellformed_\<Xi> val.\<xi>m1_matches_\<Xi>,
+   simplified, OF repeat_corres[simplified]]
 
 end
